Example4.v
@@ -8,6 +8,8 @@ Open Scope string_scope.
 Require Import ExtrOcamlBasic.
 Require Import ExtrOcamlString.
 
+Require Import Coq.ZArith.BinInt.
+
 From Verbatim Require Import regex.
 From Verbatim Require Import state.
 From Verbatim Require Import Table.
@@ -20,7 +22,6 @@ From Verbatim Require Import concrete1.
 
 From Verbatim Require Import memo.memo.
 From Verbatim Require Import memo.impl.
-From Verbatim Require Import memo.correctness.
 From Verbatim Require Import concrete3.
 
 Module Export MEM <: memo.T.
@@ -187,6 +188,100 @@ Module Export MEM <: memo.T.
       Lemma pointer_compare_trans : forall c x y z,
           pointer_compare x y = c -> pointer_compare y z = c -> pointer_compare x z = c.
       Proof. apply re_compare_trans. Qed.
+
+      Fixpoint pos2list (p : positive) : list bool :=
+        match p with
+          | xH => []
+          | xO p' => false :: (pos2list p')
+          | xI p' => true :: (pos2list p')
+        end.
+
+      Fixpoint list2pos (bs : list bool) : positive :=
+        match bs with
+        | [] => xH
+        | false :: bs' => xO (list2pos bs')
+        | true :: bs' => xI (list2pos bs')
+        end.
+
+      Lemma list_inv_pos : forall p,
+          list2pos (pos2list p) = p.
+      Proof.
+        induction p; sis; try rewrite IHp; auto.
+      Qed.
+
+      Definition int2list (z : Z) : list bool :=
+        match z with
+        | 0%Z => []
+        | Z.pos z' => true :: (pos2list z')
+        | Z.neg z' => false :: (pos2list z')
+        end.
+
+      Definition list2int (bs : list bool) : Z :=
+        match bs with
+        | [] => 0%Z
+        | true :: bs' => Z.pos (list2pos bs')
+        | false :: bs' => Z.neg (list2pos bs')
+        end.
+
+      Lemma list_inv_int : forall z,
+          list2int (int2list z) = z.
+      Proof.
+        destruct z.
+        - sis. auto.
+        - sis. rewrite list_inv_pos. auto.
+        - sis. rewrite list_inv_pos. auto.
+      Qed.
+
+      Definition index : Type := Z.
+      Definition index0 : index := 0%Z.
+
+      Lemma index_eq_dec : forall (i ii : index), {i = ii} + {i <> ii}.
+      Proof. repeat decide equality. Qed.
+      
+      Definition init_index (n : nat) : index :=
+        match n with
+        | 0 => index0
+        | S m => Z.pos (P_of_succ_nat m)
+        end.
+      
+      Definition index2list : index -> list bool:= int2list.
+      Definition list2index : list bool -> index := list2int.
+      
+      Lemma list_inv : forall (x : index), list2index (index2list x) = x.
+      Proof. apply list_inv_int. Qed.
+
+      Definition incr : index -> index := Z.succ.
+      Definition decr : index -> index := Z.pred.
+
+      (* for index correctness *)
+      Lemma decr_inv_incr : forall i, decr (incr i) = i.
+      Proof. apply Z.pred_succ. Qed.
+        
+        
+      Lemma incr_inv_decr : forall i, incr (decr i) = i.
+      Proof. apply Z.succ_pred. Qed.
+      
+      Lemma decr_inv_S : forall n, decr (init_index (S n)) = init_index n.
+      Proof.
+        induction n; auto.
+        sis. repeat dm.
+        - sis. inv E0.
+        - sis. inv E0. inv E. apply f_equal. rewrite H0. apply Pos.pred_double_succ.
+        - sis. inv E0.
+      Qed.
+      
+      Lemma incr_is_S : forall n, init_index (S n) = incr (init_index n).
+      Proof.
+        induction n; auto.
+        unfold init_index. unfold incr. apply Pos2Z.inj_succ.
+      Qed.
+      
+      Lemma n_det_index : forall n1 n2, init_index n1 = init_index n2 -> n1 = n2.
+      Proof.
+        intros. unfold init_index in *. destruct n1; destruct n2; try discriminate; auto.
+        repeat rewrite Znat.Zpos_P_of_succ_nat in H. repeat rewrite <- Znat.Nat2Z.inj_succ in *.
+        apply Znat.Nat2Z.inj; auto.
+      Qed.
       
     End Ty.
     
@@ -203,8 +298,8 @@ End MEM.
 Import MEM.STT.
 Module L := memo.impl.ImplFn MEM.
 Import L.
-Module C := memo.correctness.CorrectFn MEM.
-Import C.
+(*Module C := memo.correctness.CorrectFn MEM.
+Import C.*)
 
 Definition toS (z : string) : String := list_ascii_of_string z.
 Definition Sig_of_N (n : nat) : Sigma := ascii_of_nat 65.
@@ -306,6 +401,6 @@ Definition rus : list Rule := [ru_ws;ru_number;ru_string;ru_true;ru_false;ru_nul
 Definition lex := lex__M.
 Definition lex' := lex'__M.
 
-Extraction "Evaluation/Example/instance.ml" lex rus lex_sound__M lex_complete__M.
+Extraction "Evaluation/Example/instance.ml" lex rus.
 
 
