Verbatim/memo/concrete3.v
@@ -5,8 +5,9 @@ Require Import FSets FSets.FMapAVL FSets.FMapFacts.
 
 From Verbatim Require Import state.
 From Verbatim Require Import memo.
-From Verbatim Require Import Orders.
 From Verbatim Require Import ltac.
+From Verbatim Require Import Orders.
+From Verbatim Require Import hashtrie.
 
 
 Module FMemo (STT : state.T) <: MEMO STT.
@@ -14,42 +15,63 @@ Module FMemo (STT : state.T) <: MEMO STT.
   Import STT.Ty.
   Import STT.Defs.
   Import STT.R.Defs.
+  Import Trie.
 
   Module Pointer_as_UOT <: UsualOrderedType := UOT_from_UCT Pointer_as_UCT.
-  Module Suffix_as_UOT <: UsualOrderedType := List_as_UOT T_as_UOT.
-  Module pair_as_UOT <: UsualOrderedType := Pair_as_UOT Pointer_as_UOT Suffix_as_UOT.
-
-  Module FM := FMapAVL.Make pair_as_UOT.
+  Module FM := FMapAVL.Make Pointer_as_UOT.
   Module FMF := FMapFacts.Facts FM.
 
-  Definition Memo : Type := FM.t (option (String * String)).
-  Definition emptyMemo : Memo := FM.empty (option (String * String)).
-
-  Definition set_Memo (M : Memo) (pnt : Pointer) (sx : String) (o : (option (String * String))) :=
-    FM.add (pnt, sx) o M.
-
-  Definition get_Memo (M : Memo) (pnt : Pointer) (sx : String)
-    : option (option (String * String)) :=
-    FM.find (pnt, sx) M.
-
-
-  Lemma correct_Memo : forall M stt z o, get_Memo (set_Memo M stt z o) stt z = Some (o).
-  Proof.
-    intros. unfold get_Memo. unfold set_Memo. apply FMF.add_eq_o. auto.
-  Qed.
+  Definition Memo : Type := FM.t (@Trie (option (String * String * index))).
+  Definition emptyMemo : Memo := FM.empty (@Trie (option (String * String * index))).
   
-  Lemma correct_Memo_moot : forall M stt stt' z z' o,
-      (stt <> stt' \/ z <> z')
-      -> 
-      get_Memo (set_Memo M stt' z' o) stt z = get_Memo M stt z.
+  Definition get_Memo (M : Memo) (pnt : Pointer) (i : index)
+    : option (option (String * String * index)) :=
+    match FM.find pnt M with
+    | None => None
+    | Some T => get_Trie T (index2list i)
+    end.
+  
+  Definition set_Memo (M : Memo) (pnt : Pointer) (i : index)
+             (o : (option (String * String * index))) : Memo :=
+    match FM.find pnt M with
+    | None => FM.add pnt (set_Trie Leaf (index2list i) o) M
+    | Some T => FM.add pnt (set_Trie T (index2list i) o) M 
+    end.
+
+  Lemma correct_Memo : forall M ptr i o, get_Memo (set_Memo M ptr i o) ptr i = Some o.
   Proof.
-    intros. unfold get_Memo. unfold set_Memo. apply FMF.add_neq_o.
-    intros C. inv C. destruct H; contradiction.
+    intros. unfold get_Memo. unfold set_Memo. repeat dm.
+    - rewrite FMF.add_eq_o in E; auto. repeat inj_all. apply get_set.
+    - rewrite FMF.add_eq_o in E; auto. repeat inj_all. apply get_set.
+    - rewrite FMF.add_eq_o in E; auto. discriminate.
+    - rewrite FMF.add_eq_o in E; auto. discriminate.
+  Qed.
+
+  
+  Lemma correct_Memo_moot : forall M ptr ptr' i i' o,
+      (ptr <> ptr' \/ i <> i')
+      -> 
+      get_Memo (set_Memo M ptr' i' o) ptr i = get_Memo M ptr i.
+  Proof.
+    intros. unfold get_Memo. unfold set_Memo.
+    destruct (Pointer_as_UOT.eq_dec ptr ptr') eqn:E;
+      destruct (index_eq_dec i i'); destruct H;
+      repeat dm;
+      try(rewrite FMF.add_neq_o in *; auto; rewrite E in *; repeat inj_all; auto; discriminate);
+      try(rewrite FMF.add_eq_o in *; auto;
+          repeat inj_all; rewrite E1 in *; repeat inj_all; rewrite get_set_moot; auto;
+          intros C; destruct H; apply f_equal with (f := list2index) in C;
+          repeat rewrite list_inv in C; auto; discriminate);
+      try(try subst i; rewrite FMF.add_neq_o in *; auto; rewrite E0 in *;
+          repeat inj_all; auto; discriminate);
+      try(subst ptr; rewrite E1 in *; discriminate).
+    - rewrite FMF.add_eq_o in *; auto; discriminate.
   Qed.
     
   Lemma correct_emptyMemo : forall stt z, get_Memo emptyMemo stt z = None.
   Proof.
-    intros. unfold get_Memo. unfold emptyMemo. apply FMF.empty_o.
+    intros. unfold get_Memo. unfold emptyMemo. repeat dm.
+    rewrite FMF.empty_o in E. discriminate.
   Qed.
   
 
