fixbin/hashtrie.v
@@ -1,0 +1,63 @@
+Require Import List.
+Import ListNotations.
+
+From Verbatim Require Import ltac.
+
+
+Module Trie.
+
+  Inductive Trie {Target : Type} : Type :=
+  | Leaf
+  | Branch (t : option Target) (t0 t1 : Trie).
+
+  Fixpoint set_Trie {Target : Type} (T : Trie) (key : list bool) (value : Target) : Trie :=
+    match key with
+    | [] =>
+      match T with
+      | Leaf => Branch (Some value) Leaf Leaf
+      | Branch _ t0 t1 => Branch (Some value) t0 t1
+      end
+    | b :: bs =>
+      match T with
+      | Leaf =>
+        if b then Branch None (set_Trie Leaf bs value) Leaf
+        else Branch None Leaf (set_Trie Leaf bs value)
+      | Branch t t0 t1 =>
+        if b then Branch t (set_Trie t0 bs value) t1
+        else Branch t t0 (set_Trie t1 bs value)
+      end
+    end.
+
+  Fixpoint get_Trie {Target : Type} (T : Trie) (key : list bool) : option Target :=
+    match T with
+    | Leaf => None
+    | Branch t t0 t1 =>
+      match key with
+      | [] => t
+      | b :: bs =>
+        if b then get_Trie t0 bs
+        else get_Trie t1 bs
+      end
+    end.
+
+  Lemma get_set : forall {Target : Type} key T (value : Target),
+      get_Trie (set_Trie T key value) key = Some value.
+  Proof.
+    induction key; intros.
+    - sis. repeat dm.
+    - sis. repeat dm; sis; apply IHkey.
+  Qed.
+
+  Lemma get_set_moot : forall {Target : Type} k0 k1 (v : Target) T,
+      k0 <> k1
+      -> get_Trie (set_Trie T k0 v) k1 = get_Trie T k1.
+  Proof.
+    induction k0; destruct k1; intros.
+    - contradiction.
+    - clear H. sis. repeat dm. sis. repeat dm.
+    - clear H. sis. repeat dm.
+    - sis. repeat dm; sis; repeat dm; apply IHk0; intros C; destruct H; rewrite C; auto.
+  Qed.
+
+End Trie.
+  
